proof: Introduce some invariants

lockserver/proof.dfy
@@ -15,27 +15,6 @@ import opened Generic_Defs
 import opened System
 import opened Proof_Defs
 
-/* Safety Property: No two clients can be working on the same server */
-predicate Safety(cons:Constants, ds:DistrSys) 
-    requires cons.WF() && ds.WF(cons)
-{
-    forall i, j | 
-        && cons.ValidClientIdx(i)
-        && cons.ValidClientIdx(j)
-        && ClientIsWorking(cons, ds, i)
-        && ClientIsWorking(cons, ds, j)
-        && ds.clients[i].state.sid == ds.clients[j].state.sid
-    ::
-        i == j
-}
-
-predicate Inv(cons:Constants, ds:DistrSys) 
-{
-    && cons.WF() 
-    && ds.WF(cons)
-    && Safety(cons, ds)
-}
-
 lemma Inv_Init(cons:Constants, ds:DistrSys) 
     requires Init(cons, ds)
     ensures Inv(cons, ds)
@@ -45,5 +24,8 @@ lemma Inv_Next(cons:Constants, ds:DistrSys, ds':DistrSys)
     requires Inv(cons, ds)
     requires Next(cons, ds, ds')
     ensures Inv(cons, ds')
-{}
+{
+    // TODO
+    assume false;
+}
 }
