lockserver/proof_definitions.dfy
@@ -13,10 +13,119 @@ import opened Server_Agent
 import opened Generic_Defs
 import opened System
 
+/************************************** Properties **************************************/
+
+/* Safety Property: No two clients can be working on the same server */
+predicate Safety(cons:Constants, ds:DistrSys) 
+    requires cons.WF() && ds.WF(cons)
+{
+    forall i, j | 
+        && cons.ValidClientIdx(i)
+        && cons.ValidClientIdx(j)
+        && ClientIsWorking(cons, ds, i)
+        && ClientIsWorking(cons, ds, j)
+        && ds.clients[i].state.sid == ds.clients[j].state.sid
+    ::
+        i == j
+}
+
+/* Main Inductive Invariant */
+predicate Inv(cons:Constants, ds:DistrSys) 
+{
+    && Trivialities(cons, ds)
+    && Safety(cons, ds)
+    && ClientWorking_Implies_NoMatchingRelease(cons, ds)
+    && NoMatchingRelease_Implies_ServerLocked(cons, ds)
+    && ServerLocked_Implies_AtMostOneNonMatchedGrant(cons, ds)
+}
+
+/* Trivial parts of the main Inv */
+predicate Trivialities(cons:Constants, ds:DistrSys) {
+    && cons.WF() 
+    && ds.WF(cons)
+    && ValidPackets(cons, ds)
+}
+
+predicate ValidPackets(cons:Constants, ds:DistrSys) 
+    requires cons.WF() && ds.WF(cons)
+{
+    forall p | p in ds.network.sentPackets ::
+    match p.msg {
+        case Request(_) => ClientToServerPkt(cons, p)
+        case Release(_) => ClientToServerPkt(cons, p)
+        case Grant(_) => ServerToClientPkt(cons, p)
+        case Reject(_) => ServerToClientPkt(cons, p)
+    }
+}
+
+/* For each client c in Working(s) and epoch e, there exists a Grant(s, c, e) with no 
+matching Release */
+predicate ClientWorking_Implies_NoMatchingRelease(cons:Constants, ds:DistrSys) 
+    requires cons.WF() && ds.WF(cons)
+{
+    forall cidx | cons.ValidClientIdx(cidx) && ds.clients[cidx].state.Working? 
+    ::
+    var grant_p := Packet(ds.clients[cidx].state.sid, ds.clients[cidx].consts.id, Grant(ds.clients[cidx].epoch));
+    && grant_p in ds.network.sentPackets
+    && GetMatchingRelease(grant_p) !in ds.network.sentPackets
+}
+
+/* For each valid Grant packet, no matching release implies server is locked */
+predicate NoMatchingRelease_Implies_ServerLocked(cons:Constants, ds:DistrSys) 
+    requires cons.WF() && ds.WF(cons)
+    requires ValidPackets(cons, ds)
+{
+    forall grant_p:Packet | 
+        && IsGrantPacket(ds, grant_p)
+        && GetMatchingRelease(grant_p) !in ds.network.sentPackets
+    :: ds.servers[grant_p.src.idx].resource == Held(grant_p.dst)
+}
+
+
+/* Server locked implies at most one non-matched Grant */
+predicate ServerLocked_Implies_AtMostOneNonMatchedGrant(cons:Constants, ds:DistrSys) 
+    requires cons.WF() && ds.WF(cons)
+    requires ValidPackets(cons, ds)
+{
+    //TODO 
+    false
+}
+
+/***************************************** Utils *****************************************/
+
+/* Is this client in the Working state? */
 predicate ClientIsWorking(cons:Constants, ds:DistrSys, cidx:int)
     requires cons.WF() && ds.WF(cons)
     requires cons.ValidClientIdx(cidx)
 {
     ds.clients[cidx].state.Working?
+}
+
+/* p is a packet from a server a client */
+predicate ServerToClientPkt(cons:Constants, p:Packet)
+    requires cons.WF()
+{
+    p.src in cons.server_ids && p.dst in cons.client_ids
+}
+
+/* p is a packet from a client a server */
+predicate ClientToServerPkt(cons:Constants, p:Packet)
+    requires cons.WF()
+{
+    p.src in cons.client_ids && p.dst in cons.server_ids
+}
+
+predicate IsGrantPacket(ds:DistrSys, p:Packet) {
+    p.msg.Grant? && p in ds.network.sentPackets
+}
+
+
+
+/* Returns the corresponding Release packet for a Grant */
+function {:opaque} GetMatchingRelease(p:Packet) : (r:Packet)
+    requires p.msg.Grant?
+    ensures r == Packet(p.dst, p.src, Release(p.msg.e))
+{
+    Packet(p.dst, p.src, Release(p.msg.e))
 }
 }
